finished Mem proofs

Language_Components/Calc/Calc_Mem_Imp_Hoare.thy
@@ -50,6 +50,11 @@ definition start_state :: "syn gensyn \<Rightarrow> (syn, unit) Mem_Simple.state
   , empty
   , ())"
 
+definition state_mem where
+"state_mem st =
+  (case st of
+    (_, _, _, _, _, _, m, _) \<Rightarrow> m)"
+
 definition prog_mini :: "syn gensyn" where
 "prog_mini =  G (Sc (Cnum 42)) []
 "
@@ -115,6 +120,14 @@ value "sem_run sem_final 100 (start_state prog_mini)"
 
 value "sem_run sem_final 100 (start_state (prog1 2 3))"
 
+(* quick n dirty approach: we should be able to get this information from the liftings,
+   but this requires more machinery *)
+definition st_valid where
+"st_valid st = 
+  (case st of
+   (mdp _ (Some _), mdp _ (Some _)
+   ,mdp _ (Some _), _, _) \<Rightarrow> True
+   | _ \<Rightarrow> False)"
   
 
 (* ok great - so this finally works. now let's see if we can prove anything. *)
@@ -122,16 +135,546 @@ value "sem_run sem_final 100 (start_state (prog1 2 3))"
 declare [[show_types = false]]
 declare [[show_sorts = false]]
 
+(* individual pieces.
+*)
+
+lemma HCalc_calc :
+  assumes Hc : "c \<noteq> Cskip"
+  shows "Calc.calc_sem % {{P1}} c
+                         {{(\<lambda> st . case st of
+                              (x1, x2, x3) \<Rightarrow> 
+                              (\<exists> x3' . P1 (x1, x2, x3')) \<and>
+                              (\<forall> x3' . calc_sem c (x1, x2, x3') = st))}}"
+proof(rule HTSI)
+  fix a
+  assume H : "P1 a"
+
+  show "case calc_sem c a of (x1, x2, x3) \<Rightarrow> (\<exists>x3'. P1 (x1, x2, x3')) \<and> (\<forall>x3'. calc_sem c (x1, x2, x3') = calc_sem c a)"
+    using Hc H
+    by(cases c; cases a; auto simp add: split: prod.splits)
+qed
+
+lemma HCalc_skip :
+  shows "Calc.calc_sem % {{P1}} Cskip
+                         {{P1}}"
+proof(rule HTSI)
+  fix a
+  assume H : "P1 a"
+
+  show "P1 (calc_sem Cskip a)"
+    using H
+    by(cases a; auto simp add: split: prod.splits)
+qed
+
+lemma HCalc_Cnum :
+  shows "Calc.calc_sem % {{P1}} (Cnum i)
+         {{(\<lambda> st . 
+            case st of (c1, c2, x) \<Rightarrow> x = i \<and> (\<exists> old . P1 (c1, c2, old)))}}"
+proof(rule HTSI)
+  fix a
+  assume H : "P1 a"
+
+  show "case calc_sem (Cnum i) a of
+         (c1, c2, x) \<Rightarrow>
+           x = i \<and>
+           (\<exists>old. P1 (c1, c2, old))" using H
+    by(cases a; auto simp add: split: prod.splits)
+qed
+
+lemma HCalc_Cadd :
+  shows "Calc.calc_sem % {{P1}} (Cadd)
+         {{(\<lambda> st . 
+            case st of (c1, c2, x) \<Rightarrow> x = c1 + c2 \<and> 
+            (\<exists> old . P1 (c1, c2, old)))}}"
+proof(rule HTSI)
+  fix a
+  assume H : "P1 a"
+
+  show "case calc_sem Cadd a of
+         (c1, c2, x) \<Rightarrow>
+           x = c1 + c2 \<and>
+           (\<exists>old. P1 (c1, c2, old))" using H
+    by(cases a; auto simp add: split: prod.splits)
+qed
+
+(* HCalc_Csub *)
+lemma HCalc_Csub :
+  shows "Calc.calc_sem % {{P1}} (Csub)
+         {{(\<lambda> st . 
+            case st of (c1, c2, x) \<Rightarrow> x = c1 - c2 \<and> 
+            (\<exists> old . P1 (c1, c2, old)))}}"
+proof(rule HTSI)
+  fix a
+  assume H : "P1 a"
+
+  show "case calc_sem Csub a of
+         (c1, c2, x) \<Rightarrow>
+           x = c1 - c2 \<and>
+           (\<exists>old. P1 (c1, c2, old))" using H
+    by(cases a; auto simp add: split: prod.splits)
+qed
+
+lemma HCalc_Cmul :
+  shows "Calc.calc_sem % {{P1}} (Cmul)
+         {{(\<lambda> st . 
+            case st of (c1, c2, x) \<Rightarrow> x = c1 * c2 \<and> 
+            (\<exists> old . P1 (c1, c2, old)))}}"
+proof(rule HTSI)
+  fix a
+  assume H : "P1 a"
+
+  show "case calc_sem Cmul a of
+         (c1, c2, x) \<Rightarrow>
+           x = c1 * c2 \<and>
+           (\<exists>old. P1 (c1, c2, old))" using H
+    by(cases a; auto simp add: split: prod.splits)
+qed
+
+lemma HCond_Seqz :
+  shows "Cond.cond_sem % {{P1}} (Seqz)
+          {{(\<lambda> st . 
+              case st of (c, i) \<Rightarrow> c = encode_bool (i = 0) \<and>
+                (\<exists> old . P1 (old, i)))}}"
+proof(rule HTSI)
+  fix a
+  assume H : "P1 a"
+
+  show "case cond_sem Seqz a of
+         (c, i) \<Rightarrow>
+           c = encode_bool (i = 0) \<and>
+           (\<exists>old. P1 (old, i))" using H
+    by(cases a; auto simp add: cond_sem_def)
+qed
+
+lemma HCond_Sltz :
+  shows "Cond.cond_sem % {{P1}} (Sltz)
+          {{(\<lambda> st . 
+              case st of (c, i) \<Rightarrow> c = encode_bool (i < 0) \<and>
+                (\<exists> old . P1 (old, i)))}}"
+proof(rule HTSI)
+  fix a
+  assume H : "P1 a"
+
+  show "case cond_sem Sltz a of
+         (c, i) \<Rightarrow>
+           c = encode_bool (i < 0) \<and>
+           (\<exists>old. P1 (old, i))" using H
+    by(cases a; auto simp add: cond_sem_def)
+qed
+
+lemma HCond_Sgtz :
+  shows "Cond.cond_sem % {{P1}} (Sgtz)
+          {{(\<lambda> st . 
+              case st of (c, i) \<Rightarrow> c = encode_bool (i > 0) \<and>
+                (\<exists> old . P1 (old, i)))}}"
+proof(rule HTSI)
+  fix a
+  assume H : "P1 a"
+
+  show "case cond_sem Sgtz a of
+         (c, i) \<Rightarrow>
+           c = encode_bool (i > 0) \<and>
+           (\<exists>old. P1 (old, i))" using H
+    by(cases a; auto simp add: cond_sem_def)
+qed
+
+lemma HCond_skip :
+  shows "Cond.cond_sem % {{P1}} Sskip_cond
+                         {{P1}}"
+proof(rule HTSI)
+  fix a
+  assume H : "P1 a"
+
+  show "P1 (cond_sem Sskip_cond a)"
+    using H
+    by(cases a; auto simp add: cond_sem_def split: prod.splits)
+qed
+
+definition oalist_check' :: "('a :: linorder * 'b md_triv option md_prio) list \<Rightarrow> bool"
+  where
+"oalist_check' l =
+  list_all
+    (\<lambda> x . case x of
+      (k, mdp _ (Some (mdt _))) \<Rightarrow> True
+      | _ \<Rightarrow> False ) l"
+
+lift_definition oalist_check :: "('a :: linorder, 'b md_triv option md_prio) oalist \<Rightarrow> bool"
+is oalist_check' .
+
+fun oalist_unwrap' ::
+"('a :: linorder * 'b md_triv option md_prio) list \<Rightarrow>
+ ('a :: linorder * 'b) list option"
+where
+"oalist_unwrap' [] = Some []"
+| "oalist_unwrap' (h#t) =
+  (case h of
+    (k, mdp _ (Some (mdt v))) \<Rightarrow>
+      (case oalist_unwrap' t of
+        Some t' \<Rightarrow> Some ((k, v)#t')
+        | None \<Rightarrow> None)
+    | _ \<Rightarrow> None)"
+
+lemma oalist_unwrap'_keys :
+  "oalist_unwrap' l = Some l' \<Longrightarrow>
+   map fst l = map fst l'"
+proof(induction l arbitrary: l')
+  case Nil
+  then show ?case by auto
+next
+  case (Cons a l)
+  then show ?case 
+    by(auto split: prod.splits option.splits md_triv.splits md_prio.splits)
+qed
+
+lift_definition oalist_unwrap ::
+"('a :: linorder, 'b md_triv option md_prio) oalist \<Rightarrow> 
+ ('a :: linorder, 'b ) oalist option"
+is oalist_unwrap' 
+proof-
+  fix list :: "('a :: linorder * 'b md_triv option md_prio) list"
+  assume H : "strict_order (map fst list)"
+  
+  show "pred_option (\<lambda>xs. strict_order (map fst xs))
+        (oalist_unwrap' list)"
+    using H oalist_unwrap'_keys[of list]
+    by(auto simp add: pred_option_def)
+qed
+
+definition mem_ok :: "('s, 'x) Mem_Simple.state \<Rightarrow> bool" where
+"mem_ok st =
+  (case st of
+    ((mdp _ (Some (mdt _)))
+    , (mdp _ None)
+    , (mdp _ (Some (mdt _)))
+    , (mdp _ (Some (mdt _)))
+    , (mdp _ (Some (mdt _)))
+    , (mdp _ (Some (mdt _)))
+    , l
+    , _) \<Rightarrow> oalist_check l
+    | _ \<Rightarrow> False)"
+
+
+definition mem_unwrap :: "('s, 'x) Mem_Simple.state \<Rightarrow> Mem_Simple.state0 option"
+where
+"mem_unwrap st =
+ (case st of
+    ((mdp _ (Some (mdt _)))
+    , (mdp _ None)
+    , (mdp _ (Some (mdt reg_flag)))
+    , (mdp _ (Some (mdt reg_c)))
+    , (mdp _ (Some (mdt reg_a)))
+    , (mdp _ (Some (mdt reg_b)))
+    , l
+    , _) \<Rightarrow> 
+      (case oalist_unwrap l of
+       Some l' \<Rightarrow> Some (reg_flag, reg_c, reg_a, reg_b, l')
+       | None \<Rightarrow> None)
+    | _ \<Rightarrow> None)"
+    
+(* Mem_Read *)
+(*
+need to figure out a couple of things
+1. should we have the predicate P1 be over the inner data, or the "raw" wrapped data? 
+2. how to handle the different cases about whether there was or wasn't a value at that location before?
+   (this is more of a concern for write)
+*)
+
+lemma HMem_Sread :
+  shows "mem0_sem % {{ P1 }} (Sread s r)
+                   {{ (\<lambda> st .
+                        (case st of (reg_flag, reg_c, reg_a, reg_b, m) \<Rightarrow>
+                          (case get m s of
+                           Some v \<Rightarrow> 
+                           (case r of Reg_a \<Rightarrow> reg_a = v \<and> (\<exists> old . P1 (reg_flag, reg_c, old, reg_b, m))
+                                      | Reg_b \<Rightarrow> reg_b = v \<and> (\<exists> old . P1 (reg_flag, reg_c, reg_a, old, m))
+                                      | Reg_c \<Rightarrow> reg_c = v \<and> (\<exists> old . P1 (reg_flag, old, reg_a, reg_b, m))
+                                      | Reg_flag \<Rightarrow> reg_flag = v \<and> (\<exists> old . P1 (old, reg_c, reg_a, reg_b, m)))
+                            | None \<Rightarrow> P1 st))) }}"
+proof(rule HTSI)      
+  fix a
+  assume H : "P1 a"
+
+  obtain reg_flag reg_c reg_a reg_b m where
+    A : "a = (reg_flag, reg_c, reg_a, reg_b, m)"
+    by(cases a; auto)
+
+  obtain reg_flag' reg_c' reg_a' reg_b' m' where
+    Result : "mem0_sem (Sread s r) a = (reg_flag', reg_c', reg_a', reg_b', m')"
+    by(cases "mem0_sem (Sread s r) a"; auto)
+
+  show "case mem0_sem (Sread s r) a of
+         (reg_flag, reg_c, reg_a, reg_b, m) \<Rightarrow>
+           (case get m s of None \<Rightarrow> P1 (mem0_sem (Sread s r) a)
+             | Some v \<Rightarrow>
+                 (case r of
+                   Reg_a \<Rightarrow>
+                     reg_a = v \<and>
+                     (\<exists>old. P1 (reg_flag, reg_c, old, reg_b, m))
+                   | Reg_b \<Rightarrow>
+                       reg_b = v \<and>
+                       (\<exists>old. P1 (reg_flag, reg_c, reg_a, old, m))
+                   | Reg_c \<Rightarrow>
+                       reg_c = v \<and>
+                       (\<exists>old. P1 (reg_flag, old, reg_a, reg_b, m))
+                   | Reg_flag \<Rightarrow>
+                       reg_flag = v \<and>
+                       (\<exists>old. P1 (old, reg_c, reg_a, reg_b, m))))"
+  proof(cases "get m s")
+    case None
+
+    then show ?thesis
+      using H Result A
+      by(auto split: option.splits reg_id.splits)
+  next
+    case (Some v)
+    then show ?thesis using H Result A
+      by(auto split: option.splits reg_id.splits)
+  qed
+qed
+
+
+lemma str_ord_undo_update1 :
+  assumes H : "strict_order (map fst l)"
+  assumes Hget : "map_of l k = None"
+  shows "str_ord_delete k (str_ord_update k v l) = l"
+  using assms
+proof(induction l)
+  case Nil
+  then show ?case
+    by auto
+next
+  case (Cons h l)
+
+  obtain hk hv where Hkv : "h = (hk, hv)"
+    by(cases h; auto)
+
+  have Ord' : "strict_order (map fst l)"
+    using Cons.prems(1) strict_order_tl[of hk "map fst l"]
+    unfolding Hkv
+    by auto
+
+  show ?case
+  proof(cases "k = hk")
+    case True
+    then show ?thesis using Cons Hkv by auto
+  next
+    case False
+    then show ?thesis using Cons.prems Cons.IH[OF Ord'] Hkv
+      by(auto)
+  qed
+qed
+
+lemma undo_update1 :
+  "get m k = None \<Longrightarrow> delete k (update k v m) = m"
+  by(transfer; auto intro: str_ord_undo_update1)              
+
+lemma str_ord_undo_update2 :
+  assumes H : "strict_order (map fst l)"
+  assumes Hget : "map_of l k = Some v"
+  shows "str_ord_update k v (str_ord_update k v' l) = l"
+  using assms
+proof(induction l)
+  case Nil
+  then show ?case
+    by auto
+next
+  case (Cons h l)
+
+  obtain hk hv where Hkv : "h = (hk, hv)"
+    by(cases h; auto)
+
+  have Ord' : "strict_order (map fst l)"
+    using Cons.prems(1) strict_order_tl[of hk "map fst l"]
+    unfolding Hkv
+    by auto
+
+  show ?case
+  proof(cases "k = hk")
+    case True
+    then show ?thesis using Cons Hkv by auto
+  next
+    case False
+
+    have Hget' : "map_of l k = Some v"
+      using Cons.prems Cons.IH[OF Ord'] Hkv False
+      by(auto)
+
+    have Hget'' : "(k, v) \<in> set l"
+      using map_of_SomeD[OF Hget'] by simp
+
+    then obtain idx where Get_idx : "l ! idx = (k, v)" "idx < length l"
+      unfolding in_set_conv_nth by auto
+
+    show ?thesis 
+      using Hkv False Cons.prems strict_order_unfold[OF Cons.prems(1), of "idx + 1" 0] Get_idx
+        Cons.IH[OF Ord']
+      by(auto)
+  qed
+qed
+
+lemma undo_update2 :
+  "get m k = Some v \<Longrightarrow> update k v (update k v' m) = m"
+  by(transfer; auto intro: str_ord_undo_update2)              
+
+lemma str_ord_update_noop :
+  assumes H : "strict_order (map fst l)"
+  assumes Hget : "map_of l k = Some v"
+  shows "str_ord_update k v l = l" using assms
+proof(induction l)
+  case Nil
+  then show ?case 
+    by auto
+next
+  case (Cons h l)
+
+  obtain hk hv where Hkv : "h = (hk, hv)"
+    by(cases h; auto)
+
+  have Ord' : "strict_order (map fst l)"
+    using Cons.prems(1) strict_order_tl[of hk "map fst l"]
+    unfolding Hkv
+    by auto
+
+  show ?case
+  proof(cases "k = hk")
+    case True
+    then show ?thesis using Cons Hkv by auto
+  next
+    case False
+    have Hget' : "map_of l k = Some v"
+      using Cons.prems Cons.IH[OF Ord'] Hkv False
+      by(auto)
+
+    have Hget'' : "(k, v) \<in> set l"
+      using map_of_SomeD[OF Hget'] by simp
+
+    then obtain idx where Get_idx : "l ! idx = (k, v)" "idx < length l"
+      unfolding in_set_conv_nth by auto
+
+    show ?thesis 
+      using Hkv False Cons.prems strict_order_unfold[OF Cons.prems(1), of "idx + 1" 0] Get_idx
+        Cons.IH[OF Ord']
+      by(auto)
+  qed
+qed
+
+lemma update_noop :
+  assumes Hget : "get l k = Some v"
+  shows "update k v l = l" using assms
+  by(transfer; auto intro: str_ord_update_noop)              
+
+lemma HMem_Swrite :
+  shows "mem0_sem % {{ P1 }} (Swrite s r)
+                    {{ (\<lambda> st . 
+                        (case st of (reg_flag, reg_c, reg_a, reg_b, m) \<Rightarrow>
+                          (case r of
+                            Reg_a \<Rightarrow> get m s = Some reg_a
+                            | Reg_b \<Rightarrow> get m s = Some reg_b
+                            | Reg_c \<Rightarrow> get m s = Some reg_c
+                            | Reg_flag \<Rightarrow> get m s = Some reg_flag) \<and>
+                          (((\<exists>old. P1 (reg_flag, reg_c, reg_a, reg_b, update s old m)) \<or>
+                           (P1 (reg_flag, reg_c, reg_a, reg_b, delete s m)))))) }}"
+proof(rule HTSI)
+  fix a
+
+  assume H: "P1 a"
+
+  show "case mem0_sem (Swrite s r) a of
+         (reg_flag, reg_c, reg_a, reg_b, m) \<Rightarrow>
+           (case r of
+             Reg_a \<Rightarrow>
+               get m s = Some reg_a 
+             | Reg_b \<Rightarrow>
+                 get m s = Some reg_b
+             | Reg_c \<Rightarrow>
+                 get m s = Some reg_c
+             | Reg_flag \<Rightarrow>
+                 get m s = Some reg_flag) \<and>
+             ((\<exists>old. P1 (reg_flag, reg_c, reg_a, reg_b, update s old m)) \<or>
+             (P1 (reg_flag, reg_c, reg_a, reg_b, delete s m))) "
+  proof-
+  
+    obtain reg_flag reg_c reg_a reg_b m where
+      A : "a = (reg_flag, reg_c, reg_a, reg_b, m)"
+      by(cases a; auto)
+  
+    obtain reg_flag' reg_c' reg_a' reg_b' m' where
+      Result : "mem0_sem (Swrite s r) a = (reg_flag', reg_c', reg_a', reg_b', m')"
+      by(cases "mem0_sem (Swrite s r) a"; auto)
+  
+    show ?thesis
+    proof(cases "get m s")
+      case None
+      then show ?thesis using A Result H undo_update1[OF None]
+        by(cases r; auto simp add: get_update update_update)
+    next
+      case (Some v)
+  
+      have Conc' :
+        "P1 (reg_flag', reg_c', reg_a', reg_b', update s v m)"
+        using A Result H update_noop[OF Some]
+        by(cases r; auto simp add: get_update update_update )
+  
+      then show ?thesis using A Result H update_noop[OF Some]
+        by(cases r; auto simp add: get_update update_update; blast)
+    qed 
+  qed
+qed
+
+
 lemma prog1_spec :
   assumes Hi1 : "0 \<le> i1"
   assumes Hi2 : "0 \<le> i2"
 
-shows "|sem_final| {~ (\<lambda> _ . True) ~}
+shows "|sem_final| {~ st_valid ~}
                    [prog1 i1 i2]
-                   {~ (\<lambda> st . 
+                   {~ (\<lambda> st . st_valid st \<and>
                       (case st of
                         (x0, x1, reg_flag, reg_c, reg_a, reg_b, mem, xz) \<Rightarrow>
                           \<exists> p . get mem (STR ''acc'') = Some (mdp p (Some (mdt (i1 * i2))))))
   ~}"
+proof-
 
+  have "|sem_final| {~ st_valid ~}
+    [ G (Sc (Cnum i1)) []
+      , G (Sm (Swrite (STR ''arg1'') (Reg_c))) []
+      , G (Sc (Cnum i2)) []
+      , G (Sm (Swrite (STR ''arg2'') (Reg_c))) []
+      , G (Sc (Cnum 1)) []
+      , G (Sm (Swrite (STR ''one'') (Reg_c))) []
+      , G (Sc (Cnum 0)) []
+      , G (Sm (Swrite (STR ''acc'') (Reg_c))) [] ] 
+    {~ (\<lambda> st . st_valid st \<and> 
+          (\<exists> pi1 pi2 p1 p0 . 
+            get (state_mem st) (STR ''arg1'') = Some (mdp pi1 (Some (mdt i1))) \<and>
+            get (state_mem st) (STR ''arg2'') = Some (mdp pi2 (Some (mdt i2))) \<and>
+            get (state_mem st) (STR ''one'') = Some (mdp p1 (Some (mdt 1))) \<and>
+            get (state_mem st) (STR ''acc'') = Some (mdp p0 (Some (mdt 0))))) ~}"
+    using HxCons
+
+  proof(rule HT'I; rule_tac x = npost in exI)
+    fix npost
+    show "|#Calc_Mem_Imp.sem_final#| {#-st_valid, (npost +
+                                                npost)-#} [G (Calc_Mem_Imp.syn.Sc (Cnum i1)) [],
+                                                           G (Calc_Mem_Imp.syn.Sm (Swrite STR ''arg1'' Reg_c)) [],
+                                                           G (Calc_Mem_Imp.syn.Sc (Cnum i2)) [],
+                                                           G (Calc_Mem_Imp.syn.Sm (Swrite STR ''arg2'' Reg_c)) [],
+                                                           G (Calc_Mem_Imp.syn.Sc (Cnum 1)) [],
+                                                           G (Calc_Mem_Imp.syn.Sm (Swrite STR ''one'' Reg_c)) [],
+                                                           G (Calc_Mem_Imp.syn.Sc (Cnum 0)) [],
+                                                           G (Calc_Mem_Imp.syn.Sm (Swrite STR ''acc'' Reg_c))
+                                                            []] {#-(\<lambda>st.
+   st_valid st \<and>
+   (\<exists>pi1 pi2 p1 p0.
+       get (state_mem st) STR ''arg1'' = Some (mdp pi1 (Some (mdt i1))) \<and>
+       get (state_mem st) STR ''arg2'' = Some (mdp pi2 (Some (mdt i2))) \<and>
+       get (state_mem st) STR ''one'' = Some (mdp p1 (Some (mdt 1))) \<and>
+       get (state_mem st) STR ''acc'' = Some (mdp p0 (Some (mdt 0))))), npost-#}"
+      apply(auto)
+
+    (*
+      , G (Sm (Sread (STR ''arg2'') (Reg_c))) []
+      , G (Sb Sgtz) []
+
+*)
 end
